ecAdd partial correctness

examples/ecAdd/proofs/ecAdd.ec
@@ -17,9 +17,10 @@ admitted.
 
 lemma ecAdd_correct_1 x1_in y1_in x2_in y2_in :  
  phoare[ AlmostYul.main : 
-         arg = (x1_in,y1_in,x2_in,y2_in)  /\
-         ((x1_in = 0 /\ y1_in = 0) /\ (x2_in = 0 /\ y2_in = 0))
-             ==> res = (0,0) ] = 1%r.
+         arg = (x1_in,y1_in,x2_in,y2_in)  
+         /\ (x1_in = 0 /\ y1_in = 0) 
+         /\ (x2_in = 0 /\ y2_in = 0)
+                 ==> res = (0,0) ] = 1%r.
 proc. 
 rcondt 5. inline*. wp. skip. progress. 
 rcondf 7. inline*. wp. skip. progress.
@@ -101,8 +102,7 @@ lemma ecAdd_correct_4 x1_in y1_in x2_in y2_in :
          /\ 0 <= y2_in < AlmostYUL.N      
          /\ pointIsInCurve x1_in y1_in
          /\ pointIsInCurve x2_in y2_in
-         /\ x1_in = x2_in
-         /\ (P - y1_in) = y2
+         /\ x1_in = x2_in /\ (P - y1_in) %% P = y2
                ==> res = (0,0) ].
 proc.             
 rcondf 5. inline*. wp. skip. progress.  smt().
@@ -127,9 +127,188 @@ ecall (into_m_h x1).
 inline*. auto. progress.  qed.
 
 
+lemma nosmt div_fact (a P : int) : 0 < a < P /\ 0 <= P => !(P %| a).
+progress. smt(@Int @IntDiv dvdn_le). qed.
+
+
+
+lemma nosmt div_fact2 (a P : int) : 1 < P => coprime P a => !(P %| a).
+progress.
+have ->: a = a * 1. smt().
+case (P %| a * 1);auto.
+move => q.
+have : P %| 1.
+    apply (Gauss P a 1).     auto. auto.
+apply div_fact. progress. smt().
+qed.    
+
 
 lemma qqq (a b P : int) : (a - b) %% P = (a %% P - b %% P) %% P.
     smt(@Int @IntDiv). qed.
+
+search (%|).
+lemma nosmt oi (y1 y2 : int) : 0 <= y1 < P /\ 0 <= y2 < P => y1 <> y2 => 0 < y1 + y2 => y1^2 %% P = y2^2 %% P => y1 %% P = (P - y2) %% P.
+progress.
+have fact1 : y1^2 %% P - y2^2 %% P = 0.    smt.
+have  :  (y1^2  - y2^2) %% P  = 0. rewrite qqq. rewrite fact1. auto.
+have  ->:  (y1^2  - y2^2) = (y1 - y2) * (y1 + y2). smt.
+progress.
+rewrite - dvdzE in H6.
+have fact2 : P %| (y1 + y2). apply (Gauss P _ _ H6).
+apply prime_coprime. smt. 
+have : `|y1 - y2| < P. smt(@Int).
+progress.
+case ((y1 - y2) %% P = 0). 
+move => oo.
+have : `|y1 - y2| %% P = 0. smt (@Int @IntDiv).
+progress. apply div_fact2. smt. apply prime_coprime. smt. smt.
+auto.
+have fact4 : exists k, (y1 + y2) = k * P.
+     have d :   P %| (y1 + y2) <=> exists (q : int), y1 + y2 = q * P. apply (dvdzP P (y1 + y2)).
+       elim d. progress. apply (H7 fact2).
+elim fact4. progress.
+have o1 : k = 1. smt.
+have : P = y1 + y2. smt.
+smt.
+qed.
+
+
+
+op add_x' (x1 x2 y1 y2 : int) =  let slope = (y2 - y1) * inv P (x2 - x1) in (slope * slope - (x1 + x2)).
+op add_y' (x1 x2 y1 y2 : int) =  let slope = (y2 - y1) * inv P (x2 - x1) in
+                           (slope * (x1 - (slope * slope - (x1 + x2))) - y1).
+
+lemma ecAdd_correct_6 x1_in y1_in x2_in y2_in :  
+ hoare[ AlmostYul.main : 
+         arg = (x1_in,y1_in,x2_in,y2_in)
+         /\ 0 <= x1_in < AlmostYUL.N 
+         /\ 0 <= y1_in < AlmostYUL.N 
+         /\ 0 <= x2_in < AlmostYUL.N 
+         /\ 0 <= y2_in < AlmostYUL.N      
+         /\ pointIsInCurve x1_in y1_in
+         /\ pointIsInCurve x2_in y2_in
+
+         /\ !(x1_in = 0 /\ y1_in = 0)
+         /\ !(x2_in = 0 /\ y2_in = 0) 
+         /\ !(x1_in = x2_in /\ y1_in = y2_in)
+         /\ !(x1_in = x2_in /\ (P - y1_in) %% P = y2)
+               ==> res = (add_x' x1_in x2_in y1_in y2_in %% P, add_y' x1_in x2_in y1_in y2_in %% P) ].
+proc.             
+rcondf 5. inline*. wp. skip. progress. smt().
+rcondt 5. inline*. wp. skip. progress. 
+rcondf 7. inline*. auto. smt().
+rcondt 7. inline*. wp. skip. progress.
+rcondf 9. inline*. wp. skip. progress. smt().
+rcondt 9. inline*. auto. 
+rcondf 14. inline*. auto. smt().
+rcondf 19. inline*. auto. smt().
+rcondf 24. inline*. auto. progress. rewrite /as_bool.
+ have f: (AlmostYUL.N - y1{hr}) %% R = (AlmostYUL.N - y1{hr}). smt.
+ rewrite f f. clear f.             
+case (x1{hr} = x2{hr}). progress.
+smt. auto.             
+rcondt 24. inline*. auto. progress. rewrite /as_bool.
+rcondf 37. inline*. auto.  progress. rewrite /as_bool.
+seq 90 : (#pre). wp. skip. auto.
+if.  while (true). auto.              auto.
+skip. progress.
+seq 36 : (#pre /\ ret_bool = false).             
+inline *. seq 90 : (#pre /\ ret_bool = false). wp. skip. auto.
+wp. if.  while (true). auto.              auto.
+skip. auto. progress.
+rcondt 1. auto.
+seq 4 : ((
+   (0 <= x1_in && x1_in < AlmostYUL.N) /\
+   (0 <= y1_in && y1_in < AlmostYUL.N) /\
+   (0 <= x2_in && x2_in < AlmostYUL.N) /\
+   (0 <= y2_in && y2_in < AlmostYUL.N) /\
+   pointIsInCurve x1_in y1_in /\
+   pointIsInCurve x2_in y2_in /\
+   ! (x1_in = 0 /\ y1_in = 0) /\
+   ! (x2_in = 0 /\ y2_in = 0) /\
+   ! (x1_in = x2_in /\ y1_in = y2_in) /\ ! (x1_in = x2_in /\ (P - y1_in) %% P = y2_in)) /\
+  ret_bool = false /\ x1 = x1_in * R %% P
+  /\ y1 = y1_in * R %% P
+ /\ x2 = x2_in * R %% P
+/\ y2 = y2_in * R %% P).
+ecall (into_m_h y2_in). 
+ecall (into_m_h x2_in).
+ecall (into_m_h y1_in).                          
+ecall (into_m_h x1_in).
+skip. progress. 
+seq 6 : (#pre).
+seq 5 : (#pre). call (_:true). auto. call (_:true). auto.
+call (_:true). auto.  call (_:true). auto. call (_:true). auto. skip. progress.
+if. inline*. while (true). auto. auto. auto.
+seq 2 : (#pre /\ func492 = (y2_in - y1_in) * R %% P).
+ecall (submod_h y2 y1 P). inline*. wp. skip. progress. smt. smt. smt. smt. smt. smt.
+rewrite  - qqq. smt (@Int @IntDiv).
+seq 2 : (#pre /\ func500 = (x2_in - x1_in) * R %% P).
+ecall (submod_h x2 x1 P). inline*. wp. skip. progress. smt. smt. smt. smt. smt. smt.
+rewrite  - qqq. smt (@Int @IntDiv).
+pose slope_raw := (y2_in - y1_in) * (inv P (x2_in - x1_in)).
+seq 1 : (#pre /\ slope = slope_raw * R %% P).
+ecall (div_m_h (y2_in - y1_in) (x2_in - x1_in)). skip. progress. smt. smt.
+case (x2_in <> x1_in). progress.
+have : (x2_in - x1_in) %% P <> 0. smt.
+progress.
+have : (x2_in - x1_in) * R %% P <> 0.
+ rewrite - dvdzE.
+ case (P %| (x2_in - x1_in) * R).
+move => q.
+  have qq : P %| (x2_in - x1_in) \/ P %| R.
+  apply Euclide. auto. smt.
+elim qq. smt. apply div_fact2. smt. smt.
+smt.
+smt.
+simplify.
+     (* 
+
+y1^2 %% P = y2^2 %% P
+
+
+
+y1^2 %% P - y2^2 %% P = 0
+(y1^2 - y2^2) %% P  = 0
+y1^2 %% P = -y2^2 %% P
+(y1 - y2)(y1 + y2) %% P = 0     
+
+ *)
+move => eqq.
+have : y2_in %%P = (P - y1_in) %%P.
+apply (oi y2_in y1_in). smt. smt. smt.
+have ->: y2_in ^ 2 = y2_in * y2_in. smt.
+have ->: y1_in ^ 2 = y1_in * y1_in. smt.
+rewrite H7 H8. smt().
+smt().
+smt.
+seq 1 : (#pre /\ func510 = (slope_raw * slope_raw) * R %% P).
+ecall (mul_m_h slope_raw slope_raw). skip. progress. smt. smt. smt. smt.
+seq 2 : (#pre /\ func516 = (x1_in + x2_in) * R %% P).
+ecall (addmod_h x1 x2 P). inline*. wp. skip. progress. smt. smt. smt. smt. smt. smt.
+smt(@Int @IntDiv).
+seq 2 : (#pre /\ x3 = (slope_raw * slope_raw - (x1_in + x2_in)) * R %% P).
+ecall (submod_h func510 func516 P). inline*. wp. skip. progress. smt. smt. smt. smt. smt. smt.
+rewrite - qqq. auto. smt(@Int).
+seq 2 : (#pre /\ func532 = (x1_in - (slope_raw * slope_raw - (x1_in + x2_in))) * R %% P).
+ecall (submod_h x1 x3 P). inline*. wp. skip. progress. smt. smt. smt. smt. smt. smt.
+rewrite - qqq. smt(@Int).
+pose func532_raw := (x1_in - (slope_raw * slope_raw - (x1_in + x2_in))).
+seq 1 : (#pre /\ func528 = slope_raw * func532_raw * R %% P).
+ecall (mul_m_h slope_raw func532_raw). skip. progress. smt. smt. smt. smt.
+seq 2 : (#pre /\ y3 = ((slope_raw * func532_raw) - y1_in) * R %% P).
+ecall (submod_h func528 y1 P). inline*. wp. skip. progress. smt. smt. smt. smt. smt. smt.
+rewrite - qqq. smt(@Int).
+wp.
+ecall (outof_m_h y3).
+ecall (outof_m_h x3).
+skip. progress. smt. smt. smt. smt.
+have ->: (slope_raw * slope_raw - (x1_in + x2_in)) * R %% P * inv P R %% P
+ = (slope_raw * slope_raw - (x1_in + x2_in)) %% P. admit. smt.
+have ->: (slope_raw * func532_raw - y1_in) * R %% P * inv P R %% P
+ = (slope_raw * func532_raw - y1_in) %% P. admit.
+ smt.
+qed.
 
 
 
@@ -138,6 +317,12 @@ op add_x (x y : int) =  let slope = 3 * (x ^ 2) * inv P (2 * y) in (slope ^ 2 - 
 op add_y (x y : int) =  let slope = 3 * (x ^ 2) * inv P (2 * y) in
                         let x3 = add_x x y in (slope  * (x - x3) - y).
 
+lemma nosmt even_fact (n a : int) : n - a = a => even n .
+progress.
+have : n = 2*a.
+rewrite - H.    smt.
+move => q. rewrite q. smt.
+qed.    
 
 
 lemma ecAdd_correct_5 x1_in y1_in x2_in y2_in :  
@@ -166,9 +351,10 @@ rcondf 24. inline*. auto. progress. rewrite /as_bool.
  have f: (AlmostYUL.N - y2{hr}) %% R = (AlmostYUL.N - y2{hr}). smt.
  rewrite f f. 
  have ->: (AlmostYUL.N - y2{hr}) %% AlmostYUL.N = (AlmostYUL.N - y2{hr}). smt.
- admit.
-
-             
+ case (AlmostYUL.N - y2{hr} <> y2{hr});auto.
+  move => j.
+  have : even AlmostYUL.N. apply (even_fact AlmostYUL.N y2{hr}). auto.
+  smt.             
 rcondt 24. inline*. auto. progress. rewrite /as_bool.
 rcondf 33. inline*. auto. 
 
@@ -194,14 +380,44 @@ seq 2 : (#pre /\ func368 = (x1_squared + (x1_squared + x1_squared)) %% P). inlin
 pose x:= x2{hr} * x2{hr} * R %% P.
      have ->: (x + (x + x) %% P) %% R = (x + (x + x) %% P). smt.
              smt(@Int @IntDiv).
-seq 2 : (#pre /\ func382 = (y1_in + y1_in) * R %% P). inline*. wp.  progress. skip. progress. admit.
+seq 2 : (#pre /\ func382 = (y1_in + y1_in) * R %% P). inline*. wp.  progress. skip. progress.
+have ->: (y2{hr} * R %% P + y2{hr} * R %% P) %% R  = (y2{hr} * R %% P + y2{hr} * R %% P) . smt.
+smt(@Int @IntDiv).  
+  
 pose slope_raw := (3 * x1_squared_raw) * (inv P (y1_in + y1_in)).             
 seq 1 : (#pre /\ slope = slope_raw * R %% P).
 ecall (div_m_h (3 * x1_in * x1_in) (y1_in + y1_in)).
 skip. progress.
+have ->: (x1_squared_raw * R %% P +
+ (x1_squared_raw * R %% P + x1_squared_raw * R %% P)) %% P
+  = (x1_squared_raw * R %% P +
+ (x1_squared_raw * R %% P + x1_squared_raw * R %% P) %% P) %% P. smt(@Int @IntDiv).
+have ->: (x1_squared_raw * R %% P + x1_squared_raw * R %% P) %% P
+ = (x1_squared_raw * R + x1_squared_raw * R ) %% P. smt(@Int @IntDiv).
+ have ->: (x1_squared_raw * R %% P + (x1_squared_raw * R + x1_squared_raw * R) %% P) %%
+P = (x1_squared_raw * R + (x1_squared_raw * R + x1_squared_raw * R)) %%
+P. smt(@Int @IntDiv). smt(@Int).
 
-    admit. smt. smt. admit.  smt. rewrite /slope_raw. rewrite /x1_squared_raw. smt.
+smt. smt.
 
+have ->: (y2{hr} + y2{hr}) = 2 * y2{hr}. smt().
+ have : 2 * y2{hr} * R %% P <> 0. 
+ (* smt(@IntDiv @Int). *)
+ rewrite - dvdzE. 
+ case (P %| 2 * y2{hr} * R). move => q.
+ 
+
+  have qq : P %| 2 * y2{hr} \/ P %| R.
+  apply Euclide. auto. smt.
+  elim qq. move => zz.
+  have ww : P %| 2 \/ P %| y2{hr}.
+  apply Euclide. auto. smt.
+  elim ww. progress. apply div_fact. smt.
+  progress. apply div_fact. smt.
+  progress. apply div_fact2. smt. smt. auto.
+smt. 
+smt.
+smt. 
 seq 1 : (#pre /\ func392 = (slope_raw * slope_raw) * R %% P).
 ecall (mul_m_h slope_raw slope_raw). skip. progress. smt. smt. smt. smt.             
 seq 2 : (#pre /\ func398 = (x1_in + x1_in) * R %% P). inline*. wp. skip. progress.
@@ -243,7 +459,15 @@ smt(@Int @IntDiv).
 smt(@Int @IntDiv).                            
 smt(@Int @IntDiv).
 smt(@Int @IntDiv).
-have ->: x3_raw * R %% P * inv P R %% P = x3_raw %% P. admit.
+have ->: x3_raw * R %% P * inv P R %% P = x3_raw %% P.
+  have ->: x3_raw * R %% P * inv P R %% P
+    = x3_raw * R %% P * (inv P R %% P) %% P. smt(@Int @IntDiv).
+   have ->: x3_raw * R %% P * (inv P R %% P) %% P = (x3_raw * R  * (inv P R)) %% P.
+   smt(@Int @IntDiv).
+   have ->: (x3_raw * R  * (inv P R)) = (x3_raw * (R  * (inv P R))). smt().
+   have ->: x3_raw * (R * inv P R) %% P = x3_raw  * ((R * inv P R) %% P )  %% P. smt(@Int @IntDiv).
+   rewrite inv_ax_opp. smt. auto.
+    
 rewrite /add_x. simplify.
 rewrite /x3_raw.
 rewrite /slope_raw.
